AwsCryptographicMaterialProviders/dafny/AwsCryptographicMaterialProviders/Model/AwsCryptographyMaterialProvidersTypes.dfy
@@ -6,6 +6,7 @@ include "../../AwsCryptographyKeyStore/src/Index.dfy"
 include "../../../../AwsCryptographyPrimitives/src/Index.dfy"
 include "../../../../ComAmazonawsDynamodb/src/Index.dfy"
 include "../../../../ComAmazonawsKms/src/Index.dfy"
+include "../../../../Metrics/dafny/Metrics/src/Index.dfy"
 module {:extern "software.amazon.cryptography.materialproviders.internaldafny.types" } AwsCryptographyMaterialProvidersTypes
 {
   import opened Wrappers
@@ -15,7 +16,8 @@ module {:extern "software.amazon.cryptography.materialproviders.internaldafny.ty
   import AwsCryptographyPrimitivesTypes
   import ComAmazonawsDynamodbTypes
   import ComAmazonawsKmsTypes
-    // Generic helpers for verification of mock/unit tests.
+  import AwsCryptographyMetricsTypes
+  // Generic helpers for verification of mock/unit tests.
   datatype DafnyCallEvent<I, O> = DafnyCallEvent(input: I, output: O)
 
   // Begin Generated Types
@@ -1540,8 +1542,9 @@ module {:extern "software.amazon.cryptography.materialproviders.internaldafny.ty
     nameonly recipientKmsIdentifier: KmsKeyId
   )
   datatype MaterialProvidersConfig = | MaterialProvidersConfig (
-
-                                     )
+    nameonly loggerConfig: Option<AwsCryptographyMetricsTypes.MetricsLoggerConfig> := Option.None ,
+    nameonly logger: Option<AwsCryptographyMetricsTypes.ILogger> := Option.None
+  )
   datatype Materials =
     | Encryption(Encryption: EncryptionMaterials)
     | Decryption(Decryption: DecryptionMaterials)
@@ -1694,6 +1697,7 @@ module {:extern "software.amazon.cryptography.materialproviders.internaldafny.ty
     | AwsCryptographyPrimitives(AwsCryptographyPrimitives: AwsCryptographyPrimitivesTypes.Error)
     | ComAmazonawsDynamodb(ComAmazonawsDynamodb: ComAmazonawsDynamodbTypes.Error)
     | ComAmazonawsKms(ComAmazonawsKms: ComAmazonawsKmsTypes.Error)
+    | AwsCryptographyMetrics(AwsCryptographyMetrics: AwsCryptographyMetricsTypes.Error)
       // The Collection error is used to collect several errors together
       // This is useful when composing OR logic.
       // Consider the following method:
@@ -1741,11 +1745,22 @@ abstract module AbstractAwsCryptographyMaterialProvidersService
   function method DefaultMaterialProvidersConfig(): MaterialProvidersConfig
   method MaterialProviders(config: MaterialProvidersConfig := DefaultMaterialProvidersConfig())
     returns (res: Result<MaterialProvidersClient, Error>)
+    requires config.logger.Some? ==>
+               config.logger.value.ValidState()
+    modifies if config.logger.Some? then
+               config.logger.value.Modifies
+             else {}
     ensures res.Success? ==>
               && fresh(res.value)
-              && fresh(res.value.Modifies)
+              && fresh(res.value.Modifies
+                       - ( if config.logger.Some? then
+                             config.logger.value.Modifies
+                           else {}
+                       ) )
               && fresh(res.value.History)
               && res.value.ValidState()
+    ensures config.logger.Some? ==>
+              config.logger.value.ValidState()
 
   // Helper functions for the benefit of native code to create a Success(client) without referring to Dafny internals
   function method CreateSuccessOfClient(client: IAwsCryptographicMaterialProvidersClient): Result<IAwsCryptographicMaterialProvidersClient, Error> {
