Metrics/dafny/Metrics/src/AwsCryptographyMetricsOperations.dfy
@@ -1,0 +1,38 @@
+// Copyright Amazon.com Inc. or its affiliates. All Rights Reserved.
+// SPDX-License-Identifier: Apache-2.0
+
+include "../Model/AwsCryptographyMetricsTypes.dfy"
+
+module AwsCryptographyMetricsOperations refines AbstractAwsCryptographyMetricsOperations {
+  import UUID
+
+  datatype Config = Config(
+    nameonly MetricsLoggerConfig: MetricsLoggerConfig
+  )
+  type InternalConfig = Config
+  
+  predicate ValidInternalConfig?(config: InternalConfig)
+  {true}
+
+  function ModifiesInternalConfig(config: InternalConfig) : set<object>
+  {{}}
+
+  predicate CreateTextLoggerEnsuresPublicly(input: CreateTextLoggerInput , output: Result<CreateLoggerOutput, Error>)
+  {true}
+
+  method CreateTextLogger(config: InternalConfig, input: CreateTextLoggerInput)
+    returns (output: Result<CreateLoggerOutput, Error>)
+  {
+    var fileName;
+    if input.fileName.Some? {
+      fileName := input.fileName.value;
+    } else {
+      var fileName? := UUID.GenerateUUID();
+      fileName :- fileName?
+      // TODO create a generic error here for failing to create a text logger.
+      .MapFailure(e => Types.MetricsPutError(message := e));
+    }
+    // TODO call the create class to get us a TextLogger
+    return Failure(Error.MetricsPutError(message := "E"));
+  }
+}
