Metrics/dafny/Metrics/src/Index.dfy
@@ -1,0 +1,53 @@
+// Copyright Amazon.com Inc. or its affiliates. All Rights Reserved.
+// SPDX-License-Identifier: Apache-2.0
+
+include "../Model/AwsCryptographyMetricsTypes.dfy"
+include "AwsCryptographyMetricsOperations.dfy"
+
+module {:extern "software.amazon.cryptography.metrics.internaldafny" } Metrics refines AbstractAwsCryptographyMetricsService {
+  import Operations = AwsCryptographyMetricsOperations
+
+  function method DefaultMetricsLoggerConfig(): MetricsLoggerConfig 
+  {
+    MetricsLoggerConfig(
+      // TODO as a default use the text logger
+      // TODO write the text logger implementation
+      Logger := Option.None(),
+      PublishingCriteria := Option.Some(
+        PublishingCriteria.OperationLimit(
+          OperationLimit := OperationLimitInput(
+            endOfOperation := true
+          )
+        )
+      )
+    )
+  }
+
+  method MetricsLogger(config: MetricsLoggerConfig)
+    returns (res: Result<MetricsLoggerClient, Error>)
+    ensures res.Success? ==>
+              && res.value is MetricsLoggerClient
+  {
+    var logger := new MetricsLoggerClient(
+      Operations.Config(
+        MetricsLoggerConfig := config
+    ));
+    return Success(logger);
+  }
+
+  class MetricsLoggerClient... {
+
+    predicate ValidState()
+    {
+      && Operations.ValidInternalConfig?(config)
+      && Modifies == Operations.ModifiesInternalConfig(config) + {History}
+    }
+
+    constructor(config: Operations.InternalConfig)
+    {
+      this.config := config;
+      History := new IAwsCryptographicMetricsClientCallHistory();
+      Modifies := Operations.ModifiesInternalConfig(config) + {History};
+    }
+  }
+}
