Metrics/dafny/Metrics/Model/loggers.smithy
@@ -1,0 +1,57 @@
+namespace aws.cryptography.metrics
+
+use aws.polymorph#reference
+use aws.polymorph#positional
+use aws.polymorph#extendable
+
+@extendable
+resource Logger {
+  operations: [
+    Put,
+    Publish
+  ]
+}
+
+@reference(resource: Logger)
+structure MetricsLoggerReference {}
+
+structure CreateLoggerOutput {
+  @required
+  logger: MetricsLoggerReference
+}
+
+operation Put {
+  input: PutInput,
+  output: PutOutput,
+  errors: [MetricsPutError]
+}
+
+structure PutInput {
+  @required
+  logger: Metrics,
+
+  @required
+  message: String
+}
+
+structure PutOutput {
+}
+
+operation Publish {
+  input: PublishInput,
+  output: PublishOutput,
+  errors: [MetricsPublishError]
+}
+
+structure PublishInput {}
+
+structure PublishOutput {}
+
+operation CreateTextLogger {
+  input: CreateTextLoggerInput,
+  output: CreateLoggerOutput
+}
+
+structure CreateTextLoggerInput {
+  fileName: String
+} 
