Metrics/dafny/Metrics/Model/metrics.smithy
@@ -1,0 +1,112 @@
+namespace aws.cryptography.metrics
+
+use aws.polymorph#localService
+use aws.polymorph#reference
+use aws.polymorph#positional
+use aws.polymorph#extendable
+
+@range(min: 1)
+integer CountingNumber
+
+@aws.polymorph#localService(
+  sdkId: "MetricsLogger",
+  config: MetricsLoggerConfig
+)
+service AwsCryptographicMetrics {
+  version: "2023-04-01",
+  resources: [Logger],
+  operations: [
+    CreateTextLogger,
+    // CreateAwsCloudWatchLogger
+  ],
+  errors: [
+    MetricsPutError,
+    MetricsPublishError,
+    MetricsChainError
+  ]
+}
+
+union PublishingCriteria {
+  TimeLimit: SecondLimitInput,
+  MessageLimit: MessageLimitInput,
+  OperationLimit: OperationLimitInput,
+}
+
+structure MetricsLoggerConfig {
+  Logger: MetricsLoggerReference,
+  PublishingCriteria: PublishingCriteria 
+}
+
+structure SecondLimitInput {
+  @required
+  interval: CountingNumber,
+  @required
+  timeUnits: TimeUnits
+}
+
+structure MessageLimitInput {
+  @required
+  @range(min: 1, max: 100)
+  numberOfMessages: Integer
+}
+
+structure OperationLimitInput {
+  @required
+  endOfOperation: Boolean
+}
+
+structure Metrics {
+  @required
+  logger: MetricsLoggerReference,
+  @required
+  transactionId: String
+}
+
+operation Chain {
+  input: ChainInput,
+  output: ChainOutput,
+  errors: [MetricsChainError]
+}
+
+structure ChainInput {
+  @required
+  chainedLogger: Metrics,
+
+  @required
+  newLogger: Metrics,
+}
+
+structure ChainOutput {
+  @required
+  newChainedLogger: Metrics
+}
+
+@error("client")
+structure MetricsPutError {
+  @required
+  message: String,
+} 
+
+@error("client")
+structure MetricsChainError {
+  @required
+  message: String,
+}
+
+@error("client")
+structure MetricsPublishError {
+  @required
+  message: String
+}
+
+@enum([
+  {
+    name: "Seconds",
+    value: "Seconds",
+  },
+  {
+    name: "Milliseconds",
+    value: "Milliseconds",
+  },
+])
+string TimeUnits
